Alg/Basic.lean
@@ -2,3 +2,20 @@ theorem contrapositive {P Q : Prop} : (P → Q) -> (¬ Q → ¬ P) := by
   intro h
   intro nq p
   exact nq (h p)
+
+def left_concat_eq_append : a::as = [a] ++ as := rfl
+
+#print axioms left_concat_eq_append
+
+theorem _append_assoc (as bs cs : List α) : (as ++ bs) ++ cs = as ++ (bs ++ cs) := by
+  induction as with
+  | nil => rfl
+  | cons a as ih =>
+    repeat rw [List.cons_append]
+    congr
+
+#print axioms _append_assoc
+
+theorem _fold_append (as bs : List α) : as.append bs = as ++ bs := rfl
+
+#print axioms _append_assoc
